veric/invariants.v
@@ -1,1419 +1,217 @@
-From VST.msl Require Import ghost ghost_seplog sepalg_generators sepalg.
-From VST.veric Require Import compcert_rmaps shares own mpred ghosts.
-Require Import VST.zlist.sublist.
-Import List ListNotations.
+(* modified from iris.base_logic.lib.invariants *)
+
+From stdpp Require Export namespaces.
+From iris_ora.algebra Require Import gmap.
+From iris.proofmode Require Import proofmode.
+From VST.veric Require Export fancy_updates.
+From VST.veric Require Import wsat.
+
+(** Semantic Invariants *)
+Local Definition inv_def `{!wsatGS Σ} (N : namespace) (P : iProp Σ) : iProp Σ :=
+  □ ∀ E, ⌜↑N ⊆ E⌝ → |={E,E ∖ ↑N}=> ▷ P ∗ (▷ P ={E ∖ ↑N,E}=∗ emp).
+Local Definition inv_aux : seal (@inv_def). Proof. by eexists. Qed.
+Definition inv := inv_aux.(unseal).
+Global Arguments inv {Σ _} N P.
+Local Definition inv_unseal : @inv = @inv_def := inv_aux.(seal_eq).
+Global Instance: Params (@inv) 2 := {}.
+
+(** * Invariants *)
+Section inv.
+  Context `{!wsatGS Σ}.
+  Implicit Types i : positive.
+  Implicit Types N : namespace.
+  Implicit Types E : coPset.
+  Implicit Types P Q R : iProp Σ.
+
+  (** ** Internal model of invariants *)
+  Definition own_inv (N : namespace) (P : iProp Σ) : iProp Σ :=
+    ∃ i, ⌜i ∈ (↑N:coPset)⌝ ∧ ownI i P.
+
+  Lemma own_inv_acc E N P :
+    ↑N ⊆ E → own_inv N P ={E,E∖↑N}=∗ ▷ P ∗ (▷ P ={E∖↑N,E}=∗ emp).
+  Proof.
+    rewrite fancy_updates.ouPred_fupd_unseal /fancy_updates.ouPred_fupd_def.
+    iDestruct 1 as (i) "[%Hi #HiP]".
+    apply elem_of_subseteq_singleton in Hi.
+    rewrite {1 4}(union_difference_L (↑ N) E) // ownE_op; last set_solver.
+    rewrite {1 5}(union_difference_L {[ i ]} (↑ N)) // ownE_op; last set_solver.
+    iIntros "(Hw & [HE $] & $) !> !>".
+    iDestruct (ownI_open i with "[$Hw $HE $HiP]") as "($ & $ & HD)".
+    iIntros "HP [Hw $] !> !>". iApply (ownI_close _ P). by iFrame.
+  Qed.
+
+  Lemma fresh_inv_name (E : gset positive) N : ∃ i, i ∉ E ∧ i ∈ (↑N:coPset).
+  Proof.
+    exists (coPpick (↑ N ∖ gset_to_coPset E)).
+    rewrite -elem_of_gset_to_coPset (comm and) -elem_of_difference.
+    apply coPpick_elem_of=> Hfin.
+    eapply nclose_infinite, (difference_finite_inv _ _), Hfin.
+    apply gset_to_coPset_finite.
+  Qed.
+
+  Lemma own_inv_alloc N E P : ▷ P ={E}=∗ own_inv N P.
+  Proof.
+    rewrite fancy_updates.ouPred_fupd_unseal /fancy_updates.ouPred_fupd_def.
+    iIntros "HP [Hw $]".
+    iMod (ownI_alloc (.∈ (↑N : coPset)) P with "[$HP $Hw]")
+      as (i ?) "[$ ?]"; auto using fresh_inv_name.
+    do 2 iModIntro. iExists i. auto.
+  Qed.
+
+  (* This does not imply [own_inv_alloc] due to the extra assumption [↑N ⊆ E]. *)
+  Lemma own_inv_alloc_open N E P :
+    ↑N ⊆ E → ⊢ |={E, E∖↑N}=> own_inv N P ∗ (▷P ={E∖↑N, E}=∗ emp).
+  Proof.
+    rewrite fancy_updates.ouPred_fupd_unseal /fancy_updates.ouPred_fupd_def.
+    iIntros (Sub) "[Hw HE]".
+    iMod (ownI_alloc_open (.∈ (↑N : coPset)) P with "Hw")
+      as (i ?) "(Hw & #Hi & HD)"; auto using fresh_inv_name.
+    iAssert (ownE {[i]} ∗ ownE (↑ N ∖ {[i]}) ∗ ownE (E ∖ ↑ N))%I
+      with "[HE]" as "(HEi & HEN\i & HE\N)".
+    { rewrite -?ownE_op; [|set_solver..].
+      rewrite assoc_L -!union_difference_L //. set_solver. }
+    do 2 iModIntro. iFrame "HE\N". iSplitL "Hw HEi"; first by iApply "Hw".
+    iSplitL "Hi".
+    { iExists i. auto. }
+    iIntros "HP [Hw HE\N]".
+    iDestruct (ownI_close with "[$Hw $Hi $HP $HD]") as "[$ HEi]".
+    do 2 iModIntro. iSplitL; [|done].
+    iCombine "HEi HEN\i HE\N" as "HEN".
+    rewrite -?ownE_op; [|set_solver..].
+    rewrite assoc_L -!union_difference_L //; set_solver.
+  Qed.
+
+  Lemma own_inv_to_inv M P: own_inv M P -∗ inv M P.
+  Proof.
+    iIntros "#I". rewrite inv_unseal. iIntros "!>" (E H).
+    iPoseProof (own_inv_acc with "I") as "H"; eauto.
+  Qed.
+
+  (** ** Public API of invariants *)
+  Global Instance inv_contractive N : Contractive (inv N).
+  Proof. rewrite inv_unseal. solve_contractive. Qed.
+
+  Global Instance inv_ne N : NonExpansive (inv N).
+  Proof. apply contractive_ne, _. Qed.
+
+  Global Instance inv_proper N : Proper (equiv ==> equiv) (inv N).
+  Proof. apply ne_proper, _. Qed.
+
+  Global Instance inv_persistent N P : Persistent (inv N P).
+  Proof. rewrite inv_unseal. apply _. Qed.
+
+  Global Instance inv_affine N P : Affine (inv N P).
+  Proof. rewrite inv_unseal. apply _. Qed.
+
+  Lemma inv_alter N P Q : inv N P -∗ □ ▷ (P -∗ Q ∗ (Q -∗ P)) -∗ inv N Q.
+  Proof.
+    rewrite inv_unseal. iIntros "#HI #HPQ !>" (E H).
+    iMod ("HI" $! E H) as "[HP Hclose]".
+    iDestruct ("HPQ" with "HP") as "[$ HQP]".
+    iIntros "!> HQ". iApply "Hclose". iApply "HQP". done.
+  Qed.
+
+  Lemma inv_iff N P Q : inv N P -∗ □ ▷ (P ∗-∗ Q) -∗ inv N Q.
+  Proof.
+    iIntros "#HI #HPQ". iApply (inv_alter with "HI").
+    iIntros "!> !> HP". iSplitL "HP".
+    - by iApply "HPQ".
+    - iIntros "HQ". by iApply "HPQ".
+  Qed.
+
+  Lemma inv_alloc N E P : ▷ P ={E}=∗ inv N P.
+  Proof.
+    iIntros "HP". iApply own_inv_to_inv.
+    iApply (own_inv_alloc N E with "HP").
+  Qed.
+
+  Lemma inv_alloc_open N E P :
+    ↑N ⊆ E → ⊢ |={E, E∖↑N}=> inv N P ∗ (▷P ={E∖↑N, E}=∗ emp).
+  Proof.
+    iIntros (?). iMod own_inv_alloc_open as "[HI $]".
+    iApply own_inv_to_inv. done.
+  Qed.
+
+  Lemma inv_acc E N P :
+    ↑N ⊆ E → inv N P ={E,E∖↑N}=∗ ▷ P ∗ (▷ P ={E∖↑N,E}=∗ emp).
+  Proof.
+    rewrite inv_unseal /inv_def; iIntros (?) "#HI". by iApply "HI".
+  Qed.
+
+  Lemma inv_combine N1 N2 N P Q :
+    N1 ## N2 →
+    ↑N1 ∪ ↑N2 ⊆@{coPset} ↑N →
+    inv N1 P -∗ inv N2 Q -∗ inv N (P ∗ Q).
+  Proof.
+    rewrite inv_unseal. iIntros (??) "#HinvP #HinvQ !>"; iIntros (E ?).
+    iMod ("HinvP" with "[%]") as "[$ HcloseP]"; first set_solver.
+    iMod ("HinvQ" with "[%]") as "[$ HcloseQ]"; first set_solver.
+    iApply fupd_mask_intro; first set_solver.
+    iIntros "Hclose [HP HQ]".
+    iMod "Hclose" as "_". iMod ("HcloseQ" with "HQ") as "_". by iApply "HcloseP".
+  Qed.
+
+(*  Lemma except_0_inv N P : ◇ inv N P ⊢ inv N P.
+  Proof.
+    rewrite inv_unseal /inv_def /bi_except_0.
+    iIntros "[? | $]".
+    Search bi_later bi_affinely.
+Search bi_except_0 bi_intuitionistically.
+iIntros "#H !>" (E ?).
+    iMod "H". by iApply "H".
+  Qed.*)
+
+  (** ** Proof mode integration *)
+(*  Global Instance is_except_0_inv N P : IsExcept0 (inv N P).
+  Proof. apply except_0_inv. Qed.*)
+
+  Global Instance into_inv_inv N P : IntoInv (inv N P) N := {}.
+
+  Global Instance into_acc_inv N P E:
+    IntoAcc (X := unit) (inv N P)
+            (↑N ⊆ E) emp (fupd E (E ∖ ↑N)) (fupd (E ∖ ↑N) E)
+            (λ _ : (), (▷ P)%I) (λ _ : (), (▷ P)%I) (λ _ : (), None).
+  Proof.
+    rewrite /IntoAcc /accessor bi.exist_unit.
+    iIntros (?) "#Hinv _". by iApply inv_acc.
+  Qed.
+
+  (** ** Derived properties *)
+  Lemma inv_acc_strong E N P :
+    ↑N ⊆ E → inv N P ={E,E∖↑N}=∗ ▷ P ∗ ∀ E', ▷ P ={E',↑N ∪ E'}=∗ emp.
+  Proof.
+    iIntros (?) "Hinv".
+    iPoseProof (inv_acc (↑ N) N with "Hinv") as "H"; first done.
+    rewrite difference_diag_L.
+    iPoseProof (fupd_mask_frame_r _ _ (E ∖ ↑ N) with "H") as "H"; first set_solver.
+    rewrite left_id_L -union_difference_L //. iMod "H" as "[$ H]"; iModIntro.
+    iIntros (E') "HP".
+    iPoseProof (fupd_mask_frame_r _ _ E' with "(H HP)") as "H"; first set_solver.
+    by rewrite left_id_L.
+  Qed.
+
+  Lemma inv_acc_timeless E N P `{!Timeless P} :
+    ↑N ⊆ E → inv N P ={E,E∖↑N}=∗ P ∗ (P ={E∖↑N,E}=∗ emp).
+  Proof.
+    iIntros (?) "Hinv". iMod (inv_acc with "Hinv") as "[>HP Hclose]"; auto.
+    iIntros "!> {$HP} HP". iApply "Hclose"; auto.
+  Qed.
+
+  Lemma inv_split_l N P Q : inv N (P ∗ Q) -∗ inv N P.
+  Proof.
+    iIntros "#HI". iApply inv_alter; eauto.
+    iIntros "!> !> [$ $] $".
+  Qed.
+  Lemma inv_split_r N P Q : inv N (P ∗ Q) -∗ inv N Q.
+  Proof.
+    rewrite (comm _ P Q). eapply inv_split_l.
+  Qed.
+  Lemma inv_split N P Q : inv N (P ∗ Q) -∗ inv N P ∗ inv N Q.
+  Proof.
+    iIntros "#H".
+    iPoseProof (inv_split_l with "H") as "$".
+    iPoseProof (inv_split_r with "H") as "$".
+  Qed.
+
+End inv.
 
-Section Invariants.
-
-#[global] Program Instance unit_PCM : Ghost := { valid a := True; Join_G a b c := True }.
-Next Obligation.
-  apply fsep_sep, _.
-Defined.
-
-Definition pred_of (P : mpred) := SomeP rmaps.Mpred (fun _ => P).
-
-Definition agree g (P : mpred) : mpred := own(RA := unit_PCM) g tt (pred_of P).
-
-Lemma agree_dup : forall g P, (agree g P = agree g P * agree g P)%pred.
-Proof.
-  intros; apply ghost_op; constructor.
-Qed.
-
-Lemma agree_join : forall g P1 P2, agree g P1 * agree g P2 |-- (|> P1 -* |> P2) * agree g P1.
-Proof.
-  intros.
-  intros ? (? & ? & ? & H1 & H2).
-  do 3 eexists; [apply id_core_unit|].
-  pose proof (ghost_of_join _ _ _ H) as J.
-  change (agree g P1) with (own.own(RA := unit_PCM) g tt (pred_of P1)) in H1.
-  destruct H1 as (? & Hid & ? & H1).
-  change (agree g P2) with (own.own(RA := unit_PCM) g tt (pred_of P2)) in H2.
-  destruct H2 as (? & ? & ? & H2).
-  rewrite ghost_fmap_singleton in H1, H2.
-  destruct (join_assoc (join_comm H1) J) as (? & J1 & ?).
-  destruct (join_assoc (join_comm H2) (join_comm J1)) as (? & J2 & ?).
-  apply singleton_join_inv in J2 as ([] & J2 & ?); subst.
-  inv J2; simpl in *.
-  destruct H6 as [Heq1 ?].
-  apply SomeP_inj in Heq1.
-  destruct (join_level _ _ _ H) as [Hl1 Hl2]; erewrite Hl1, Hl2 in *.
-  assert (approx (level a) P1 = approx (level a) P2) as Heq.
-  { apply (@equal_f _ _ (fun _ : list Type => approx (level a) P1) (fun _ : list Type => approx (level a) P2));
-      auto.
-    apply nil. }
-  clear J.
-  split.
-  - intros ??? Hl J HP1 ? Ha'.
-    pose proof (id_core_level a).
-    pose proof (necR_level _ _ Hl).
-    apply nec_identity in Hl; [|apply id_core_identity].
-    destruct (join_level _ _ _ J).
-    apply Hl in J; subst.
-    specialize (HP1 _ Ha').
-    apply laterR_level in Ha'.
-    assert ((approx (level a) P1) a') as HP1'.
-    { split; auto; lia. }
-    rewrite Heq in HP1'; destruct HP1'; auto.
-  - exists I; split.
-    + intro l; simpl.
-      apply (resource_at_join _ _ _ l) in H.
-      apply Hid in H as <-; auto.
-    + rewrite ghost_fmap_singleton; simpl.
-      eapply join_sub_trans; [|eexists; apply join_comm; eauto].
-      eexists; eauto.
-      replace _ with I in J1 by (apply proof_irr); eauto.
-Qed.
-
-Lemma agree_join2 : forall g P1 P2, agree g P1 * agree g P2 |-- (|> P1 -* |> P2) * agree g P2.
-Proof.
-  intros.
-  intros ? (? & ? & ? & H1 & H2).
-  do 3 eexists; [apply id_core_unit|].
-  pose proof (ghost_of_join _ _ _ H) as J.
-  change (agree g P1) with (own.own(RA := unit_PCM) g tt (pred_of P1)) in H1.
-  destruct H1 as (? & Hid & ? & H1).
-  change (agree g P2) with (own.own(RA := unit_PCM) g tt (pred_of P2)) in H2.
-  destruct H2 as (? & ? & ? & H2).
-  rewrite ghost_fmap_singleton in H1, H2.
-  destruct (join_assoc (join_comm H1) J) as (? & J1 & ?).
-  destruct (join_assoc (join_comm H2) (join_comm J1)) as (? & J2 & ?).
-  apply singleton_join_inv in J2 as ([] & J2 & ?); subst.
-  inv J2; simpl in *.
-  destruct H6 as [Heq1 ?].
-  apply SomeP_inj in Heq1.
-  destruct (join_level _ _ _ H) as [Hl1 Hl2]; erewrite Hl1, Hl2 in *.
-  assert (approx (level a) P1 = approx (level a) P2) as Heq.
-  { apply (@equal_f _ _ (fun _ : list Type => approx (level a) P1) (fun _ : list Type => approx (level a) P2));
-      auto.
-    apply nil. }
-  clear J.
-  split.
-  - intros ??? Hl J HP1 ? Ha'.
-    pose proof (id_core_level a).
-    pose proof (necR_level _ _ Hl).
-    apply nec_identity in Hl; [|apply id_core_identity].
-    destruct (join_level _ _ _ J).
-    apply Hl in J; subst.
-    specialize (HP1 _ Ha').
-    apply laterR_level in Ha'.
-    assert ((approx (level a) P1) a') as HP1'.
-    { split; auto; lia. }
-    rewrite Heq in HP1'; destruct HP1'; auto.
-  - exists I; split.
-    + intro l; simpl.
-      apply (resource_at_join _ _ _ l) in H.
-      apply Hid in H as <-; auto.
-    + rewrite ghost_fmap_singleton; simpl.
-      eapply join_sub_trans; [|eexists; apply join_comm, ghost_of_join; eauto].
-      eexists; eauto.
-      replace _ with I in H2 by (apply proof_irr); eauto.
-Qed.
-
-Inductive list_join {P : Ghost} : Join (list (option G)) :=
-  | list_join_nil_l m: list_join nil m m
-  | list_join_nil_r m: list_join m nil m
-  | list_join_cons a1 a2 m1 m2 a3 m3: join a1 a2 a3 -> list_join m1 m2 m3 ->
-      list_join (a1 :: m1) (a2 :: m2) (a3 :: m3).
-#[global] Existing Instance list_join.
-
-Lemma list_join_inv: forall {P : Ghost} (l1 l2 l3 : list (option G)), list_join l1 l2 l3 ->
-match l1, l2 with
-| nil, _ => l3 = l2
-| _, nil => l3 = l1
-| a1 :: l1, a2 :: l2 => match l3 with nil => False
-                        | a3 :: l3 => join a1 a2 a3 /\ list_join l1 l2 l3 end
-end.
-Proof.
-  induction 1; simpl; auto.
-  destruct m; simpl; auto.
-Qed.
-
-#[global] Program Instance list_PCM (P : Ghost) : Ghost := { valid a := True; Join_G := list_join }.
-Next Obligation.
-Proof.
-  intros; exists (fun _ => nil); auto; intros; repeat econstructor.
-Defined.
-Next Obligation.
-Proof.
-  constructor.
-    + intros until 1.
-      revert z'; induction H; inversion 1; auto; subst.
-      f_equal; eauto.
-      eapply join_eq; eauto.
-    + induction a; intros ???? J1 J2; eapply list_join_inv in J1; subst.
-      { exists e; split; auto; constructor. }
-      destruct b; subst; [eexists; split; eauto; constructor|].
-      destruct d; [contradiction|].
-      destruct J1 as [Jc1 J1].
-      apply list_join_inv in J2.
-      destruct c; subst; [eexists; split; eauto; constructor; auto|].
-      destruct e; [contradiction|].
-      destruct J2 as [Jc2 J2].
-      destruct (join_assoc Jc1 Jc2) as (f & ? & ?).
-      destruct (IHa _ _ _ _ J1 J2) as (f' & ? & ?).
-      exists (f :: f'); split; constructor; auto.
-    + induction 1; constructor; auto.
-    + intros until 1.
-      revert b'; induction H; inversion 1; auto; subst.
-      f_equal; eauto.
-      eapply join_positivity; eauto.
-Qed.
-
-Definition ghost_list {P : Ghost} g l := own(RA := list_PCM P) g l NoneP.
-
-Definition list_singleton {A} n (a : A) := repeat None n ++ [Some a].
-
-Definition list_incl {A} (l1 l2 : list (option A)) := (length l1 <= length l2)%nat /\
-  forall n a, nth n l1 None = Some a -> nth n l2 None = Some a.
-
-(* up *)
-Lemma app_nth : forall {A} n l1 l2 (d : A),
-  nth n (l1 ++ l2) d = if lt_dec n (length l1) then nth n l1 d else nth (n - length l1) l2 d.
-Proof.
-  intros.
-  if_tac; [rewrite app_nth1 | rewrite app_nth2]; auto; lia.
-Qed.
-
-Fixpoint replace_nth {A} (n: nat) (al: list A) (x: A) {struct n}: list A :=
- match n, al with
- | O , a::al => x::al
- | S n', a::al' => a :: replace_nth n' al' x
- | _, nil => nil
- end.
-
-Lemma replace_nth_length : forall {A} n l (a : A),
-  length (replace_nth n l a) = length l.
-Proof.
-  induction n; destruct l; simpl; intros; try lia.
-  erewrite IHn by lia; auto.
-Qed.
-
-Lemma replace_nth_app : forall {A} n l1 l2 (a : A),
-  replace_nth n (l1 ++ l2) a = if lt_dec n (length l1) then replace_nth n l1 a ++ l2
-  else l1 ++ replace_nth (n - length l1) l2 a.
-Proof.
-  induction n; destruct l1; auto; simpl; intros.
-  rewrite IHn.
-  if_tac; if_tac; auto; lia.
-Qed.
-
-Lemma list_join_app : forall {P : Ghost} l1 l2 m1 m2 n1 n2,
-  length l1 = length m1 -> length l1 = length n1 ->
-  list_join l1 m1 n1 -> list_join l2 m2 n2 ->
-  list_join (l1 ++ l2) (m1 ++ m2) (n1 ++ n2).
-Proof.
-  induction 3.
-  - destruct m; auto; discriminate.
-  - destruct m; auto; discriminate.
-  - simpl in *.
-    intros; constructor; auto.
-Qed.
-
-Lemma list_join_None : forall {P : Ghost} n l, (n <= length l)%nat ->
-  list_join (repeat None n) l l.
-Proof.
-  induction n; [constructor|].
-  destruct l; simpl; [lia|].
-  repeat constructor.
-  apply IHn; lia.
-Qed.
-
-Lemma list_join_over : forall {P : Ghost} l l1 l2 l1', (length l <= length l1)%nat ->
-  list_join l l1 l1' -> list_join l (l1 ++ l2) (l1' ++ l2).
-Proof.
-  induction 2; simpl in *.
-  - constructor.
-  - destruct m; [constructor | simpl in *; lia].
-  - constructor; auto.
-    apply IHlist_join; lia.
-Qed.
-
-Lemma singleton_length : forall {A} n (a : A), length (list_singleton n a) = S n.
-Proof.
-  intros; unfold list_singleton.
-  erewrite app_length, repeat_length; simpl; lia.
-Qed.
-
-Lemma list_join_singleton : forall {P : Ghost} n a c l
-  (Hn : (n < length l)%nat) (Hjoin: join (Some a) (nth n l None) (Some c)),
-  list_join (list_singleton n a) l (replace_nth n l (Some c)).
-Proof.
-  induction l using rev_ind; simpl; intros; try lia.
-  rewrite app_length in Hn; simpl in Hn.
-  destruct (eq_dec n (length l)).
-  - subst.
-    erewrite app_nth2, Nat.sub_diag in Hjoin by lia; simpl in Hjoin.
-    erewrite replace_nth_app, if_false, Nat.sub_diag by lia; simpl.
-    apply list_join_app; try (rewrite repeat_length; auto).
-    + apply list_join_None; auto.
-    + repeat constructor; auto.
-  - assert (n < length l)%nat by lia.
-    erewrite app_nth1 in Hjoin by auto.
-    erewrite replace_nth_app, if_true by auto.
-    apply list_join_over, IHl; auto.
-    rewrite singleton_length; lia.
-Qed.
-
-(* up *)
-Lemma replace_nth_same : forall {A} n l (d : A), replace_nth n l (nth n l d) = l.
-Proof.
-  induction n; destruct l; auto; simpl; intro.
-  rewrite IHn; auto.
-Qed.
-
-Lemma nth_replace_nth : forall {A} n l a (d : A), (n < length l)%nat ->
-  nth n (replace_nth n l a) d = a.
-Proof.
-  induction n; destruct l; auto; simpl; intros; try lia.
-  apply IHn; lia.
-Qed.
-
-Lemma nth_replace_nth' : forall {A} n m l a (d : A), m <> n ->
-  nth m (replace_nth n l a) d = nth m l d.
-Proof.
-  induction n; destruct l; auto; destruct m; auto; simpl; intros; try lia.
-  apply IHn; lia.
-Qed.
-
-Lemma Znth_replace_nth : forall {A} {d : Inhabitant A} n l (a : A), (n < length l)%nat ->
-  Znth (Z.of_nat n) (replace_nth n l a) = a.
-Proof.
-  intros; rewrite <- nth_Znth'.
-  apply nth_replace_nth; auto.
-Qed.
-
-Lemma Znth_replace_nth' : forall {A} {d : Inhabitant A} n m l (a : A), m <> Z.of_nat n ->
-  Znth m (replace_nth n l a) = Znth m l.
-Proof.
-  intros.
-  destruct (zlt m 0); [rewrite !Znth_underflow; auto|].
-  rewrite <- (Z2Nat.id m) by lia.
-  rewrite <- !nth_Znth'; apply nth_replace_nth'.
-  intro; contradiction H; subst.
-  erewrite Z2Nat.id by lia; auto.
-Qed.
-
-Lemma replace_nth_replace_nth: forall {A: Type} R n {Rn Rn': A},
-  replace_nth n (replace_nth n R Rn) Rn' = replace_nth n R Rn'.
-Proof.
-  intros.
-  revert R; induction n; destruct R; simpl in *.
-  + reflexivity.
-  + reflexivity.
-  + reflexivity.
-  + rewrite IHn.
-    reflexivity.
-Qed.
-
-Lemma ghost_list_nth : forall {P : Ghost} g n l (a : G) (Ha : nth n l None = Some a),
-  (ghost_list g l = ghost_list g (list_singleton n a) * ghost_list g (replace_nth n l None))%pred.
-Proof.
-  intros; apply ghost_op.
-  rewrite <- (replace_nth_same n l None) at 2.
-  destruct (lt_dec n (length l)); [|erewrite nth_overflow in Ha by lia; discriminate].
-  exploit (list_join_singleton n a a (replace_nth n l None)).
-  { rewrite replace_nth_length; auto. }
-  { erewrite nth_replace_nth by auto; constructor. }
-  erewrite replace_nth_replace_nth, Ha; auto.
-Qed.
-
-Lemma list_join_length : forall {P : Ghost} l1 l2 l3, list_join l1 l2 l3 ->
-  (length l1 <= length l3)%nat.
-Proof.
-  induction 1; auto; simpl; lia.
-Qed.
-
-Lemma list_join_filler : forall {P : Ghost} l1 l2 l3 n, list_join l1 l2 l3 ->
-  (n <= length l3 - length l1)%nat -> list_join (l1 ++ repeat None n) l2 l3.
-Proof.
-  induction 1; simpl; intros.
-  - apply list_join_None; lia.
-  - destruct n; [|lia].
-    rewrite app_nil_r; constructor.
-  - constructor; auto.
-Qed.
-
-Lemma list_join_nth : forall {P : Ghost} l1 l2 l3 n, list_join l1 l2 l3 ->
-  join (nth n l1 None) (nth n l2 None) (nth n l3 None).
-Proof.
-  intros; revert n.
-  induction H; intro.
-  - erewrite nth_overflow by (simpl; lia); constructor.
-  - erewrite (nth_overflow []) by (simpl; lia); constructor.
-  - destruct n; simpl; auto.
-Qed.
-
-Lemma list_join_max : forall {P : Ghost} l1 l2 l3, list_join l1 l2 l3 ->
-  length l3 = Nat.max (length l1) (length l2).
-Proof.
-  induction 1; simpl; auto.
-  rewrite Nat.max_l; auto; lia.
-Qed.
-
-Lemma list_join_nth_error : forall {P : Ghost} l1 l2 l3 n, list_join l1 l2 l3 ->
-  join (nth_error l1 n) (nth_error l2 n) (nth_error l3 n).
-Proof.
-  intros; revert n.
-  induction H; intro.
-  - rewrite nth_error_nil; constructor.
-  - rewrite nth_error_nil; constructor.
-  - destruct n; simpl; auto.
-    constructor; auto.
-Qed.
-
-Lemma list_join_alt : forall {P : Ghost} l1 l2 l3,
-  list_join l1 l2 l3 <-> forall n, join (nth_error l1 n) (nth_error l2 n) (nth_error l3 n).
-Proof.
-  split; [intros; apply list_join_nth_error; auto|].
-  revert l2 l3; induction l1; simpl; intros.
-  - assert (l2 = l3); [|subst; constructor].
-    apply list_nth_error_eq; intro.
-    specialize (H j); rewrite nth_error_nil in H; inv H; auto.
-  - destruct l2.
-    + assert (a :: l1 = l3); [|subst; constructor].
-      apply list_nth_error_eq; intro.
-      specialize (H j); rewrite nth_error_nil in H; inv H; auto.
-    + destruct l3.
-      { specialize (H O); inv H. }
-      constructor.
-      * specialize (H O); inv H; auto.
-      * apply IHl1; intro.
-        apply (H (S n)).
-Qed.
-
-Lemma nth_error_replace_nth : forall {A} n l (a : A), (n < length l)%nat ->
-  nth_error (replace_nth n l a) n = Some a.
-Proof.
-  induction n; destruct l; auto; simpl; intros; try lia.
-  apply IHn; lia.
-Qed.
-
-Lemma nth_error_replace_nth' : forall {A} n m l (a : A), m <> n ->
-  nth_error (replace_nth n l a) m = nth_error l m.
-Proof.
-  induction n; destruct l; auto; destruct m; auto; simpl; intros; try lia.
-  apply IHn; lia.
-Qed.
-
-#[global] Instance list_order A : @PCM_order (list_PCM (discrete_PCM A)) list_incl.
-Proof.
-  constructor.
-  - constructor.
-    + repeat intro; split; auto.
-    + repeat intro.
-      destruct H, H0; split; auto; lia.
-  - intro a.
-    remember (length a) as n.
-    revert dependent a; induction n; intros.
-    + destruct a; inv Heqn.
-      exists b; split; auto.
-      change [] with (core b); apply core_unit.
-    + assert (a <> []) by (intro; subst; discriminate).
-      erewrite (app_removelast_last None) in H, Heqn by auto.
-      erewrite app_length in Heqn; simpl in Heqn.
-      erewrite Nat.add_1_r in Heqn; inv Heqn.
-      specialize (IHn _ eq_refl).
-      destruct (IHn b c) as (c' & ? & ?); auto.
-      { destruct H as [Hlen H].
-        split.
-        { rewrite app_length in Hlen; simpl in *; lia. }
-        intros ?? Hnth.
-        specialize (H n a0).
-        rewrite app_nth in H.
-        if_tac in H; auto.
-        rewrite nth_overflow in Hnth; [discriminate|].
-        apply not_lt; auto. }
-      pose proof (list_join_length _ _ _ H2).
-      pose proof (list_join_length _ _ _ (join_comm H2)).
-      destruct (eq_dec (length (removelast a)) (length c')).
-      * exists (c' ++ [List.last a None]); split.
-        -- erewrite (app_removelast_last None) at 1 by auto.
-           apply join_comm, list_join_over; try lia.
-           apply join_comm in H2; auto.
-        -- split.
-            { destruct H.
-              erewrite app_length in *; simpl in *; lia. }
-            intros ?? Hnth.
-            rewrite app_nth in Hnth.
-            if_tac in Hnth; [apply H3; auto|].
-            destruct (n - length c')%nat eqn: Hminus; [|destruct n0; discriminate].
-            simpl in Hnth.
-            apply H.
-            erewrite app_nth2 by lia.
-            replace (_ - _)%nat with O by lia; auto.
-       * destruct (List.last a None) eqn: Ha.
-         -- exists (replace_nth (length (removelast a)) c' (Some g)).
-            split.
-            ++ apply list_join_alt; intro.
-               pose proof (list_join_max _ _ _ H2) as Hlen.
-               destruct (Nat.max_spec (length (removelast a)) (length b)) as [[? Hmax] | [? Hmax]];
-                 setoid_rewrite Hmax in Hlen; try lia.
-               hnf in H2; erewrite list_join_alt in H2.
-               specialize (H2 n0).
-               erewrite (app_removelast_last None) at 1 by auto.
-               rewrite Ha.
-               destruct (lt_dec n0 (length (removelast a))).
-               ** erewrite nth_error_app1 by auto.
-                  erewrite nth_error_replace_nth' by lia; auto.
-               ** erewrite nth_error_app2 by lia.
-                  destruct (eq_dec n0 (length (removelast a))).
-                  { subst; rewrite Nat.sub_diag; simpl.
-                    erewrite nth_error_replace_nth by (simpl in *; lia).
-                    destruct (nth_error b (length (removelast a))) eqn: Hb; setoid_rewrite Hb; constructor.
-                    destruct o; constructor.
-                    destruct H0 as [_ Hc].
-                    erewrite sublist.nth_error_nth in Hb by lia.
-                    inv Hb.
-                    apply Hc in H7.
-                    destruct H as [_ Hc'].
-                    specialize (Hc' (length (removelast a))).
-                    erewrite app_nth2, Nat.sub_diag in Hc' by auto.
-                    setoid_rewrite Hc' in H7; [|reflexivity].
-                    inv H7; constructor; auto. }
-                  { destruct (_ - _)%nat eqn: Hminus; [lia | simpl].
-                    erewrite nth_error_nil, nth_error_replace_nth' by (simpl in *; lia).
-                    destruct (nth_error_length n0 (removelast a)) as [_ Hnone].
-                    setoid_rewrite Hnone in H2; [auto | lia]. }
-            ++ destruct H3.
-               split.
-               { rewrite replace_nth_length; auto. }
-               intros ?? Hnth.
-               destruct (eq_dec n0 (length (removelast a)));
-                 [|rewrite nth_replace_nth' in Hnth; auto].
-               subst; erewrite nth_replace_nth in Hnth by (simpl in *; lia).
-               inv Hnth.
-               apply H.
-               erewrite app_nth2, Nat.sub_diag; auto.
-         -- exists c'; split; auto.
-            erewrite (app_removelast_last None), Ha by auto.
-            apply @list_join_filler with (n := 1%nat); auto; simpl in *; lia.
-  - split.
-    + split; [eapply list_join_length; eauto|].
-      intros ?? Hnth.
-      apply @list_join_nth with (n := n) in H.
-      rewrite Hnth in H; inv H; auto.
-      inv H3; auto.
-    + split; [apply join_comm in H; eapply list_join_length; eauto|].
-      intros ?? Hnth.
-      apply @list_join_nth with (n := n) in H.
-      rewrite Hnth in H; inv H; auto.
-      inv H3; auto.
-  - induction a; unfold list_incl; intros.
-    + destruct b; [constructor|].
-      simpl in *; lia.
-    + destruct H as [? Hnth].
-      destruct b; constructor.
-      * destruct o; [|constructor].
-        specialize (Hnth O _ eq_refl); simpl in Hnth.
-        subst; repeat constructor.
-      * apply IHa.
-        split; [simpl in *; lia|].
-        intros.
-        apply (Hnth (S n)); auto.
-Qed.
-
-(*Notation union := base.union.
-
-#[global] Program Instance set_PCM : Ghost := { valid := fun _ : coPset => True;
-  Join_G a b c := a ## b /\ c = union a b(*; core2 a := empty*) }.
-Next Obligation.
-Proof.
-  exists (fun _ => empty); auto.
-  intro; split; set_solver.
-Defined.
-Next Obligation.
-  constructor.
-    + intros.
-      inv H; inv H0; auto.
-    + intros.
-      inv H; inv H0.
-      eexists; split; [split; eauto | split]; set_solver.
-    + intros.
-      inv H.
-      split; set_solver.
-    + intros.
-      inv H; inv H0.
-      set_solver.
-Qed.*)
-
-Import Ensembles.
-
-Lemma Union_comm: forall {A} S T, Union A S T = Union A T S.
-Proof.
-  intros; extensionality; apply prop_ext; split; intro H; inv H; solve [constructor 1; auto] || solve [constructor 2; auto].
-Qed.
-
-Lemma Union_assoc: forall {A} S T U, Union A (Union A S T) U = Union A S (Union A T U).
-Proof.
-  intros; extensionality; apply prop_ext; split; intro H; inv H.
-  - inv H0; [constructor 1 | constructor 2; constructor 1]; auto.
-  - constructor 2; constructor 2; auto.
-  - constructor 1; constructor 1; auto.
-  - inv H0; [constructor 1; constructor 2 | constructor 2]; auto.
-Qed.
-
-Lemma Union_Empty : forall {A} S, Union A (Empty_set A) S = S.
-Proof.
-  intros; extensionality; apply prop_ext; split; intro H.
-  - inv H; auto; contradiction.
-  - constructor 2; auto.
-Qed.
-
-Lemma Intersection_comm: forall {A} S T, Intersection A S T = Intersection A T S.
-Proof.
-  intros; extensionality; apply prop_ext; split; intro H; inv H; constructor; auto.
-Qed.
-
-Lemma Intersection_assoc: forall {A} S T U, Intersection A (Intersection A S T) U = Intersection A S (Intersection A T U).
-Proof.
-  intros; extensionality; apply prop_ext; split; intro H; inv H.
-  - inv H0; repeat constructor; auto.
-  - inv H1; repeat constructor; auto.
-Qed.
-
-Lemma Intersection_Empty : forall {A} S, Intersection A (Empty_set A) S = Empty_set A.
-Proof.
-  intros; extensionality; apply prop_ext; split; intro H; inv H; auto.
-Qed.
-
-Global Arguments Union {_} _ _.
-Global Arguments Intersection {_} _ _.
-Global Arguments Disjoint {_} _ _.
-Global Arguments Add {_} _ _.
-Global Arguments Setminus {_} _ _.
-Global Arguments Subtract {_} _ _.
-Global Arguments Full_set {_}.
-Global Arguments Empty_set {_}.
-Global Arguments Singleton {_} _.
-Global Arguments In {_} _ _.
-Global Arguments Included {_} _ _.
-Global Arguments Same_set {_} _ _.
-
-#[global] Polymorphic Program Instance set_PCM : Ghost := { valid := fun _ : Ensemble nat => True;
-  Join_G a b c := Disjoint a b /\ c = Union a b }.
-Next Obligation.
-Proof.
-  apply fsep_sep; exists (fun _ => Empty_set); auto.
-  intro; split.
-  - constructor; intros ? X.
-    rewrite Intersection_Empty in X; contradiction.
-  - rewrite Union_Empty; auto.
-Defined.
-Next Obligation.
-  constructor.
-    + intros ???? [] []; subst; auto.
-    + intros ????? [Hd1] [Hd2]; subst.
-      inv Hd1; inv Hd2.
-      exists (Union b c); repeat (split; auto).
-      * intros ? X; inv X.
-        contradiction (H0 x).
-        constructor; auto.
-        right; auto.
-      * intros ? X; inv X.
-        inv H2.
-        -- contradiction (H x); constructor; auto.
-        -- contradiction (H0 x); constructor; auto.
-           left; auto.
-      * apply Union_assoc.
-    + intros ??? []; subst.
-      split.
-      * inv H; constructor.
-        intros x X; inv X; contradiction (H0 x); constructor; auto.
-      * apply Union_comm.
-    + intros ???? [] []; subst.
-      extensionality; apply prop_ext; split; intro X.
-      { left; auto. }
-      rewrite H2; left; auto.
-Qed.
-
-Definition ghost_set g s := own(RA := set_PCM) g s NoneP.
-
-Lemma ghost_set_join : forall g s1 s2,
-  (ghost_set g s1 * ghost_set g s2 = !!(Disjoint s1 s2) && ghost_set g (Union s1 s2))%pred.
-Proof.
-  intros.
-  setoid_rewrite own_op_gen.
-  - instantiate (1 := Union s1 s2).
-    unfold ghost_set; apply pred_ext.
-    + apply prop_andp_left; intros (? & (? & []) & ?).
-      apply prop_andp_right; auto.
-    + apply prop_andp_left; intros.
-      apply prop_andp_right; auto.
-      eexists; repeat (split; auto).
-  - intros (? & H & ?); inv H; split; auto.
-Qed.
-
-Lemma ghost_set_subset : forall g s s' (Hdec : forall a, In s' a \/ ~In s' a),
-  (Included s' s -> ghost_set g s = ghost_set g s' * ghost_set g (Setminus s s'))%pred.
-Proof.
-  intros.
-  apply ghost_op.
-  split.
-  - constructor; intros ? X; inv X.
-    inv H1; contradiction.
-  - extensionality; apply prop_ext; split; intro X.
-    + destruct (Hdec x); [left | right; constructor]; auto.
-    + destruct X. apply H; auto. inv H0; auto.
-Qed.
-
-Corollary ghost_set_remove : forall g a s,
-  In s a -> (ghost_set g s = ghost_set g (Singleton a) * ghost_set g (Subtract s a))%pred.
-Proof.
-  intros; apply ghost_set_subset.
-  { intro b; destruct (eq_dec a b); [left; subst; constructor | right; intros X; inv X; contradiction]. }
-  intros ? X; inv X; auto.
-Qed.
-
-Definition iname := nat.
-
-Class invG := { g_inv : gname; g_en : gname; g_dis : gname }.
-
-Context {inv_names : invG}.
-
-Definition master_list {A} g (l : list (option A)) := ghost_master1(ORD := list_order A) l g.
-
-(* Our ghost state construction makes it awkward to put agree inside other ghost state constructions.
-   As a workaround, instead of having one ghost location with a map from indices to agrees,
-   we have a map from indices to ghost locations, each with an agree. *)
-
-#[global] Instance token_PCM : Ghost := exclusive_PCM unit.
-
-Fixpoint iter_sepcon {A} (p : A -> mpred) l :=
-  match l with
-    | nil => emp
-    | x :: xl => (p x * iter_sepcon p xl)%pred
-  end.
-
-Typeclasses eauto := 1.
-
-#[global] Instance Inhabitant_mpred : Inhabitant mpred := emp.
-
-Definition wsat : mpred := (EX I : list mpred, EX lg : list gname, EX lb : list (option bool),
-  !!(length lg = length I /\ length lb = length I) &&
-  master_list g_inv (map (fun i => match Znth i lb with Some _ => Some (Znth i lg)
-                                   | None => None end) (upto (length I))) *
-  ghost_list g_dis (map (fun o => match o with Some true => Some (Some tt) | _ => None end) lb) *
-  ghost_set g_en (fun i : iname => nth i lb None = Some false) *
-  iter_sepcon (fun i => match Znth i lb with
-                        | Some true => agree (Znth i lg) (Znth i I) * |> Znth i I
-                        | Some false => agree (Znth i lg) (Znth i I)
-                        | _ => emp end) (upto (length I)))%pred.
-
-(* This is what's called ownI in Iris; we could build another layer with namespaces. *)
-Definition invariant (i : iname) P : mpred := (EX g : gname,
-  ghost_snap(ORD := list_order _) (list_singleton i g) g_inv * agree g P)%pred.
-
-Lemma nth_singleton : forall {A} n (a : A) d, nth n (list_singleton n a) d = Some a.
-Proof.
-  intros; unfold list_singleton.
-  rewrite app_nth2; rewrite repeat_length; auto.
-  rewrite Nat.sub_diag; auto.
-Qed.
-
-Lemma list_join_singleton_inv : forall {P : Ghost} n a b l,
-  list_join (list_singleton n a) (list_singleton n b) l ->
-  exists c, join a b c /\ l = list_singleton n c.
-Proof.
-  induction n; inversion 1; subst.
-  - inv H5.
-    inv H6; eauto.
-  - edestruct IHn as (c & ? & ?); eauto; subst.
-    inv H5; eauto.
-Qed.
-
-Lemma singleton_join_self : forall {P: Ghost} k (a : G), join a a a ->
-  join (list_singleton k a) (list_singleton k a) (list_singleton k a).
-Proof.
-  intros.
-  induction k; repeat constructor; auto.
-Qed.
-
-Lemma invariant_dup : forall i P, (invariant i P = invariant i P * invariant i P)%pred.
-Proof.
-  intros; unfold invariant; apply pred_ext.
-  - apply exp_left; intro g.
-    rewrite exp_sepcon1; apply exp_right with g.
-    rewrite exp_sepcon2; apply exp_right with g.
-    rewrite <- sepcon_assoc, (sepcon_comm _ (ghost_snap _ _)), <- sepcon_assoc.
-    erewrite ghost_snap_join.
-    erewrite sepcon_assoc, <- agree_dup; apply derives_refl.
-    { apply (singleton_join_self(P := discrete_PCM _)).
-      constructor; auto. }
-  - rewrite exp_sepcon1; apply exp_left; intro g1.
-    rewrite exp_sepcon2; apply exp_left; intro g2.
-    erewrite <- sepcon_assoc, (sepcon_comm _ (ghost_snap _ _)), <- sepcon_assoc.
-    rewrite ghost_snap_join'.
-    rewrite !exp_sepcon1; apply exp_left; intro l.
-    rewrite !sepcon_andp_prop1; apply prop_andp_left; intro H.
-    apply (list_join_singleton_inv(P := discrete_PCM _)) in H as (g & H & ?); subst.
-    inv H.
-    erewrite sepcon_assoc, <- agree_dup.
-    apply exp_right with g; apply derives_refl.
-Qed.
-
-(* up *)
-Lemma Zlength_eq : forall {A B} (l1 : list A) (l2 : list B),
-  Zlength l1 = Zlength l2 <-> length l1 = length l2.
-Proof.
-  intros; rewrite !Zlength_correct.
-  split; [apply Nat2Z.inj|].
-  intro; apply Z2Nat.inj; try lia.
-Qed.
-
-#[global] Instance list_Perm {P : Ghost} : Perm_alg (list (option G)).
-Proof.
-  apply list_PCM.
-Qed.
-
-(* up *)
-Lemma nth_upto : forall m n d, (n < m)%nat -> nth n (upto m) d = Z.of_nat n.
-Proof.
-  intros.
-  erewrite nth_indep by (rewrite upto_length; auto).
-  erewrite nth_Znth', Znth_upto; auto.
-  split; [lia|].
-  apply Nat2Z.inj_lt; auto.
-Qed.
-
-Lemma nth_repeat : forall {A} n m (a : A), nth n (repeat a m) a = a.
-Proof.
-  induction n; destruct m; simpl; auto.
-Qed.
-
-Lemma list_incl_singleton : forall {A} n (a : A) l,
-  list_incl (list_singleton n a) l <-> nth n l None = Some a.
-Proof.
-  unfold list_incl; split.
-  - intros [? Hnth].
-    apply Hnth.
-    rewrite nth_singleton; auto.
-  - intros; split.
-    + rewrite singleton_length.
-      destruct (lt_dec n (length l)); [lia|].
-      erewrite nth_overflow in H by lia; discriminate.
-    + intros ??.
-      unfold list_singleton.
-      destruct (lt_dec n0 n).
-      * erewrite app_nth1 by (rewrite repeat_length; auto).
-        rewrite nth_repeat; discriminate.
-      * rewrite app_nth2; rewrite repeat_length; try lia.
-        destruct (eq_dec n0 n); [|erewrite nth_overflow by (simpl; lia); discriminate].
-        subst; rewrite Nat.sub_diag; simpl.
-        intro X; inv X; auto.
-Qed.
-
-Lemma seq_app : forall a b c, seq a (b + c) = seq a b ++ seq (a + b) c.
-Proof.
-  intros ??; revert a; induction b; simpl; intros; auto.
-  rewrite IHb; do 3 f_equal; lia.
-Qed.
-
-Lemma filter_ext_in : forall {A} (f g : A -> bool) l, (forall x, List.In x l -> f x = g x) -> filter f l = filter g l.
-Proof.
-  induction l; auto; simpl; intros.
-  rewrite -> H by auto.
-  rewrite IHl; auto.
-Qed.
-
-Lemma filter_none : forall {A} (f : A -> bool) l, (forall x, List.In x l -> f x = false) -> filter f l = [].
-Proof.
-  induction l; auto; simpl; intros.
-  rewrite H; auto.
-Qed.
-
-Ltac view_shift H := eapply derives_trans; [apply sepcon_derives, derives_refl; apply H
-  | eapply derives_trans; [apply bupd_frame_r | eapply derives_trans, bupd_trans; apply bupd_mono]].
-
-Lemma iter_sepcon_app:
-  forall {B} p (l1 l2 : list B), (iter_sepcon p (l1 ++ l2) = iter_sepcon p l1 * iter_sepcon p l2)%pred.
-Proof.
-  induction l1; intros; simpl. rewrite emp_sepcon; auto. rewrite IHl1. rewrite sepcon_assoc. auto.
-Qed.
-
-Lemma iter_sepcon_func_strong: forall {A} (l : list A) P Q, (forall x, List.In x l -> P x = Q x) -> iter_sepcon P l = iter_sepcon Q l.
-Proof.
-  intros. induction l.
-  + reflexivity.
-  + simpl.
-    f_equal.
-    - apply H.
-      simpl; auto.
-    - apply IHl.
-      intros; apply H.
-      simpl; auto.
-Qed.
-
-Lemma iter_sepcon_emp': forall {B} p (l : list B), (forall x, List.In x l -> p x = emp) -> iter_sepcon p l = emp.
-Proof.
-  induction l; intros; simpl; auto.
-  rewrite H, IHl, sepcon_emp; simpl; auto.
-  intros; apply H; simpl; auto.
-Qed.
-
-Lemma wsat_alloc_dep : forall P, wsat * (ALL i, |> P i) |-- |==> wsat * EX i : _, invariant i (P i).
-Proof.
-  intros; unfold wsat.
-  rewrite !exp_sepcon1; apply exp_left; intro l.
-  rewrite !exp_sepcon1; apply exp_left; intro lg.
-  rewrite !exp_sepcon1; apply exp_left; intro lb.
-  rewrite !sepcon_andp_prop1; apply prop_andp_left; intros [].
-  rewrite (sepcon_comm _ (ghost_list _ _)), !sepcon_assoc.
-  view_shift (ghost_update_ND(RA := list_PCM token_PCM) g_dis (map
-     (fun o => match o with Some true => Some (Some tt) | _ => None end) lb)
-     (fun l => exists i, l =
-      map (fun o => match o with Some true => Some (Some tt) | _ => None end)
-          ((lb ++ repeat None i) ++ [Some true]))).
-  { intros ? (? & ? & _).
-    exists (map (fun o => match o with Some true => Some (Some tt) | _ => None end)
-      ((lb ++ repeat None (length x - length lb)) ++ [Some true])).
-    split; [eauto|].
-    exists (x ++ [Some (Some tt)]); split; simpl; auto.
-    erewrite !map_app, own.map_repeat; simpl.
-    pose proof (list_join_length _ _ _ H1) as Hlen.
-    rewrite map_length in Hlen.
-    apply join_comm in H1.
-    pose proof (list_join_length _ _ _ H1) as Hlen'.
-    apply (join_comm(Perm_alg := list_Perm)), (list_join_over c).
-    { erewrite app_length, map_length, repeat_length, Nat.add_comm, Nat.sub_add; auto. }
-    apply (join_comm(Perm_alg := list_Perm)), (list_join_filler(P := token_PCM));
-      [|rewrite map_length; auto].
-    apply join_comm in H1; auto. }
-  rewrite exp_sepcon1; apply exp_left; intro.
-  rewrite !sepcon_andp_prop1; apply prop_andp_left; intros [i ?]; subst.
-  eapply derives_trans with (emp * _)%pred; [rewrite emp_sepcon; apply derives_refl|].
-  set (P' := P (length lg + i)%nat).
-  view_shift (ghost_alloc(RA := unit_PCM) tt (pred_of P')); [simpl; auto|].
-  rewrite !exp_sepcon1; apply exp_left; intro g.
-  replace (own(RA := unit_PCM) g tt (pred_of P')) with (agree g P') by reflexivity.
-  rewrite agree_dup.
-  assert (Zlength lg = Zlength l) as Hlg by (apply Zlength_eq; auto).
-  assert (Zlength lb = Zlength l) as Hlb by (apply Zlength_eq; auto).
-  rewrite <- !sepcon_assoc, (sepcon_comm _ (master_list _ _)), !sepcon_assoc.
-  view_shift (master_update(ORD := list_order _) ((map (fun i0 : Z =>
-      match Znth i0 lb with Some _ => Some (Znth i0 lg) | None => None end) (upto (Datatypes.length l))))
-        (map (fun j => match Znth j ((lb ++ repeat None i) ++ [Some true]) with
-                       | Some _ => Some (Znth j ((lg ++ repeat O i) ++ [g]))
-                       | None => None
-                       end) (upto (length ((l ++ repeat emp i) ++ [P']))))).
-  { rewrite <- !app_assoc, app_length, upto_app, map_app.
-    split.
-    { erewrite app_length, !map_length; lia. }
-    intros ?? Hn.
-    erewrite app_nth, map_length.
-    if_tac; [|erewrite nth_overflow in Hn by (rewrite map_length; lia); discriminate].
-    erewrite nth_map' with (d' := 0) in * by auto.
-    erewrite upto_length in *.
-    assert (Z.of_nat n < Zlength l).
-    { rewrite Zlength_correct; apply Nat2Z.inj_lt; auto. }
-    erewrite nth_upto in * by auto.
-    erewrite !app_Znth1 by lia; auto. }
-  view_shift (make_snap(ORD := list_order gname)).
-  rewrite !sepcon_assoc.
-  view_shift (ghost_snap_forget(ORD := list_order _) (list_singleton (length lg + i) g)).
-  { apply list_incl_singleton.
-    erewrite app_length, upto_app, map_app, app_nth2; erewrite map_length, upto_length, app_length,
-      repeat_length; try lia.
-    replace (_ - _)%nat with O by lia; simpl.
-    rewrite Nat2Z.inj_add, Z.add_0_r.
-    rewrite !app_Znth2; erewrite !Zlength_app, !coqlib4.Zlength_repeat, <- Zlength_correct; try lia.
-    replace (_ - _) with 0 by lia; replace (_ - _) with 0 by lia; auto. }
-  eapply derives_trans, bupd_intro.
-  apply exp_right with ((l ++ repeat emp i) ++ [P']).
-  rewrite exp_sepcon1; apply exp_right with ((lg ++ repeat O i) ++ [g]).
-  rewrite exp_sepcon1; apply exp_right with ((lb ++ repeat None i) ++ [Some true]).
-  erewrite !(app_length (_ ++ _)); simpl.
-  erewrite prop_true_andp by (erewrite !app_length, !repeat_length; lia).
-  erewrite upto_app, iter_sepcon_app; simpl.
-  erewrite Z.add_0_r, <- Zlength_correct, !app_Znth2; erewrite !Zlength_app, !coqlib4.Zlength_repeat; try lia.
-  erewrite Hlg, Hlb, Zminus_diag, !Znth_0_cons.
-  rewrite sepcon_comm, !sepcon_assoc; apply sepcon_derives; [apply derives_refl|].
-  rewrite <- sepcon_assoc, sepcon_comm, sepcon_assoc; apply sepcon_derives; [apply derives_refl|].
-  rewrite sepcon_assoc; apply sepcon_derives.
-  { match goal with |-?P |-- ?Q => replace P with Q; [apply derives_refl|] end.
-    f_equal. extensionality; apply prop_ext; split; intro X.
-    - rewrite !app_nth, nth_repeat in X.
-      repeat destruct (lt_dec _ _); auto; try discriminate.
-      destruct (x - _)%nat; [|destruct n0]; inv X.
-    - destruct (lt_dec x (length lb)).
-      rewrite !app_nth, app_length.
-      destruct (lt_dec _ _); [|lia].
-      destruct (lt_dec _ _); [auto | lia].
-      { rewrite nth_overflow in X by lia; discriminate. } }
-  erewrite app_length, upto_app, iter_sepcon_app.
-  rewrite sepcon_assoc; apply sepcon_derives.
-  - eapply derives_trans with (_ * emp)%pred; [rewrite sepcon_emp; apply derives_refl|].
-    apply sepcon_derives.
-    + erewrite iter_sepcon_func_strong; auto.
-      intros ??%In_upto.
-      rewrite <- Zlength_correct in *.
-      rewrite <- !app_assoc, !app_Znth1 by (rewrite ?Zlength_app; lia); auto.
-    + rewrite iter_sepcon_emp'; auto.
-      intros ? Hin.
-      eapply in_map_iff in Hin as (? & ? & Hin%In_upto); subst.
-      rewrite <- Zlength_correct, coqlib4.Zlength_repeat in Hin.
-      rewrite <- Zlength_correct, <- app_assoc, app_Znth2 by lia.
-      erewrite app_Znth1 by (rewrite coqlib4.Zlength_repeat; lia).
-      unfold Znth; destruct (Z_lt_dec _ _); auto.
-      rewrite nth_repeat; auto.
-  - unfold invariant.
-    rewrite emp_sepcon, !exp_sepcon2; apply exp_right with (length lg + i)%nat.
-    rewrite !exp_sepcon2; apply exp_right with g.
-    rewrite <- !sepcon_assoc, sepcon_comm, !sepcon_assoc; apply sepcon_derives; [apply derives_refl|].
-    apply sepcon_derives, derives_refl.
-    eapply allp_left, derives_refl.
-Qed.
-
-Lemma wsat_alloc : forall P, wsat * |> P |-- |==> wsat * EX i : _, invariant i P.
-Proof.
-  intros; eapply derives_trans, wsat_alloc_dep.
-  apply sepcon_derives; [apply derives_refl|].
-  apply allp_right; auto.
-Qed.
-
-(* request an iname with a particular property *)
-Lemma wsat_alloc_strong : forall P Pi (Hfresh : forall n, exists i, (n <= i)%nat /\ Pi i),
-  wsat * |> P |-- |==> wsat * EX i : _, !!(Pi i) && invariant i P.
-Proof.
-  intros; unfold wsat.
-  rewrite !exp_sepcon1; apply exp_left; intro l.
-  rewrite !exp_sepcon1; apply exp_left; intro lg.
-  rewrite !exp_sepcon1; apply exp_left; intro lb.
-  rewrite !sepcon_andp_prop1; apply prop_andp_left; intros [].
-  rewrite (sepcon_comm _ (ghost_list _ _)), !sepcon_assoc.
-  view_shift (ghost_update_ND(RA := list_PCM token_PCM) g_dis (map
-     (fun o => match o with Some true => Some (Some tt) | _ => None end) lb)
-     (fun l => exists i, Pi (length lg + i)%nat /\ l =
-      map (fun o => match o with Some true => Some (Some tt) | _ => None end)
-          ((lb ++ repeat None i) ++ [Some true]))).
-  { intros ? (? & ? & _).
-    destruct (Hfresh (length x)) as (i & ? & ?).
-    exists (map (fun o => match o with Some true => Some (Some tt) | _ => None end)
-      ((lb ++ repeat None (i - length lb)) ++ [Some true])).
-    pose proof (list_join_length _ _ _ H1) as Hlen.
-    rewrite map_length in Hlen.
-    split.
-    { exists (i - length lg)%nat; rewrite H, H0; split; auto.
-      rewrite Nat.add_comm, Nat.sub_add; auto; lia. }
-    exists (x ++ repeat None (i - length x) ++ [Some (Some tt)]); split; simpl; auto.
-    erewrite !map_app, own.map_repeat; simpl.
-    apply join_comm in H1.
-    rewrite app_assoc; apply (join_comm(Perm_alg := list_Perm)), (list_join_over c).
-    { apply list_join_length in H1.
-      rewrite app_length, map_length, repeat_length, Nat.add_comm, Nat.sub_add; auto; lia. }
-    replace (i - length lb)%nat with ((length x - length lb) + (i - length x))%nat by lia.
-    rewrite repeat_app, app_assoc; apply (list_join_over c).
-    { apply list_join_length in H1.
-      rewrite app_length, map_length, repeat_length; lia. }
-    apply (join_comm(Perm_alg := list_Perm)), (list_join_filler(P := token_PCM));
-      [|rewrite map_length; auto].
-    apply join_comm in H1; auto. }
-  rewrite exp_sepcon1; apply exp_left; intro.
-  rewrite !sepcon_andp_prop1; apply prop_andp_left; intros [i []]; subst.
-  eapply derives_trans with (emp * _)%pred; [rewrite emp_sepcon; apply derives_refl|].
-  view_shift (ghost_alloc(RA := unit_PCM) tt (pred_of P)); [simpl; auto|].
-  rewrite !exp_sepcon1; apply exp_left; intro g.
-  replace (own(RA := unit_PCM) g tt (pred_of P)) with (agree g P) by reflexivity.
-  rewrite agree_dup.
-  assert (Zlength lg = Zlength l) as Hlg by (apply Zlength_eq; auto).
-  assert (Zlength lb = Zlength l) as Hlb by (apply Zlength_eq; auto).
-  rewrite <- !sepcon_assoc, (sepcon_comm _ (master_list _ _)), !sepcon_assoc.
-  view_shift (master_update(ORD := list_order _) ((map (fun i0 : Z =>
-      match Znth i0 lb with Some _ => Some (Znth i0 lg) | None => None end) (upto (Datatypes.length l))))
-        (map (fun j => match Znth j ((lb ++ repeat None i) ++ [Some true]) with
-                       | Some _ => Some (Znth j ((lg ++ repeat O i) ++ [g]))
-                       | None => None
-                       end) (upto (length ((l ++ repeat emp i) ++ [P]))))).
-  { rewrite <- !app_assoc, app_length, upto_app, map_app.
-    split.
-    { erewrite app_length, !map_length; lia. }
-    intros ?? Hn.
-    erewrite app_nth, map_length.
-    if_tac; [|erewrite nth_overflow in Hn by (rewrite map_length; lia); discriminate].
-    erewrite nth_map' with (d' := 0) in * by auto.
-    erewrite upto_length in *.
-    assert (Z.of_nat n < Zlength l).
-    { rewrite Zlength_correct; apply Nat2Z.inj_lt; auto. }
-    erewrite nth_upto in * by auto.
-    erewrite !app_Znth1 by lia; auto. }
-  view_shift (make_snap(ORD := list_order gname)).
-  rewrite !sepcon_assoc.
-  view_shift (ghost_snap_forget(ORD := list_order _) (list_singleton (length lg + i) g)).
-  { apply list_incl_singleton.
-    erewrite app_length, upto_app, map_app, app_nth2; erewrite map_length, upto_length, app_length,
-      repeat_length; try lia.
-    replace (_ - _)%nat with O by lia; simpl.
-    rewrite Nat2Z.inj_add, Z.add_0_r.
-    rewrite !app_Znth2; erewrite !Zlength_app, !coqlib4.Zlength_repeat, <- Zlength_correct; try lia.
-    replace (_ - _) with 0 by lia; replace (_ - _) with 0 by lia; auto. }
-  eapply derives_trans, bupd_intro.
-  apply exp_right with ((l ++ repeat emp i) ++ [P]).
-  rewrite exp_sepcon1; apply exp_right with ((lg ++ repeat O i) ++ [g]).
-  rewrite exp_sepcon1; apply exp_right with ((lb ++ repeat None i) ++ [Some true]).
-  erewrite !(app_length (_ ++ _)); simpl.
-  erewrite prop_true_andp by (erewrite !app_length, !repeat_length; lia).
-  erewrite upto_app, iter_sepcon_app; simpl.
-  erewrite Z.add_0_r, <- Zlength_correct, !app_Znth2; erewrite !Zlength_app, !coqlib4.Zlength_repeat; try lia.
-  erewrite Hlg, Hlb, Zminus_diag, !Znth_0_cons.
-  rewrite sepcon_comm, !sepcon_assoc; apply sepcon_derives; [apply derives_refl|].
-  rewrite <- sepcon_assoc, sepcon_comm, sepcon_assoc; apply sepcon_derives; [apply derives_refl|].
-  rewrite sepcon_assoc; apply sepcon_derives.
-  { match goal with |-?P |-- ?Q => replace P with Q; [apply derives_refl|] end.
-    f_equal. extensionality; apply prop_ext; split; intro X.
-    - rewrite !app_nth, nth_repeat in X.
-      repeat destruct (lt_dec _ _); auto; try discriminate.
-      destruct (x - _)%nat; [|destruct n0]; inv X.
-    - destruct (lt_dec x (length lb)).
-      rewrite !app_nth, app_length.
-      destruct (lt_dec _ _); [|lia].
-      destruct (lt_dec _ _); [auto | lia].
-      { rewrite nth_overflow in X by lia; discriminate. } }
-  erewrite app_length, upto_app, iter_sepcon_app.
-  rewrite sepcon_assoc; apply sepcon_derives.
-  - eapply derives_trans with (_ * emp)%pred; [rewrite sepcon_emp; apply derives_refl|].
-    apply sepcon_derives.
-    + erewrite iter_sepcon_func_strong; auto.
-      intros ??%In_upto.
-      rewrite <- Zlength_correct in *.
-      rewrite <- !app_assoc, !app_Znth1 by (rewrite ?Zlength_app; lia); auto.
-    + rewrite iter_sepcon_emp'; auto.
-      intros ? Hin.
-      eapply in_map_iff in Hin as (? & ? & Hin%In_upto); subst.
-      rewrite <- Zlength_correct, coqlib4.Zlength_repeat in Hin.
-      rewrite <- Zlength_correct, <- app_assoc, app_Znth2 by lia.
-      erewrite app_Znth1 by (rewrite coqlib4.Zlength_repeat; lia).
-      unfold Znth; destruct (Z_lt_dec _ _); auto.
-      rewrite nth_repeat; auto.
-  - unfold invariant.
-    rewrite emp_sepcon, !exp_sepcon2; apply exp_right with (length lg + i)%nat.
-    rewrite prop_true_andp by auto.
-    rewrite !exp_sepcon2; apply exp_right with g.
-    rewrite <- !sepcon_assoc, sepcon_comm, !sepcon_assoc; apply derives_refl.
-Qed.
-
-Lemma iter_sepcon_Znth: forall {A} {d : Inhabitant A} f (l : list A) i, 0 <= i < Zlength l ->
-  iter_sepcon f l = (f (Znth i l) * iter_sepcon f (remove_Znth i l))%pred.
-Proof.
-  intros; unfold remove_Znth.
-  transitivity (iter_sepcon f (sublist 0 (Zlength l) l)); [rewrite sublist_same; auto|].
-  rewrite sublist_split with (mid := i) by lia.
-  rewrite (sublist_next i) by lia.
-  rewrite !iter_sepcon_app; simpl.
-  rewrite <- !sepcon_assoc, (sepcon_comm (f _)); reflexivity.
-Qed.
-
-Lemma map_replace_nth:
-  forall {A B} (f: A -> B) n R X, map f (replace_nth n R X) =
-       replace_nth n (map f R) (f X).
-Proof.
-  intros.
-  revert R; induction n; destruct R; simpl; auto.
-  f_equal; auto.
-Qed.
-
-Lemma wsat_open : forall i P,
-  (wsat * invariant i P * ghost_set g_en (Singleton i) |--
-  |==> wsat * |> P * ghost_list g_dis (list_singleton i (Some tt))).
-Proof.
-  intros; unfold wsat, invariant.
-  rewrite !exp_sepcon1; apply exp_left; intros l.
-  rewrite !exp_sepcon1; apply exp_left; intros lg.
-  rewrite !exp_sepcon1; apply exp_left; intros lb.
-  rewrite !sepcon_andp_prop1; apply prop_andp_left; intros [].
-  rewrite !exp_sepcon2, exp_sepcon1; apply exp_left; intros g.
-  eapply derives_trans, (prop_andp_left (i < length lg /\ Znth (Z.of_nat i) lg = g /\
-    exists b, Znth (Z.of_nat i) lb = Some b)%nat).
-  { rewrite <- sepcon_assoc, (sepcon_comm _ (ghost_snap _ _)), <- !sepcon_assoc.
-    unfold master_list; rewrite snap_master_join1.
-    rewrite !sepcon_andp_prop1; apply andp_derives, derives_refl.
-    apply prop_derives; intros Hincl.
-    apply list_incl_singleton in Hincl.
-    destruct (lt_dec i (length lg));
-      [|rewrite nth_overflow in Hincl by (rewrite map_length, upto_length; lia); discriminate].
-    rewrite nth_map' with (d' := 0) in Hincl by (rewrite upto_length; lia).
-    rewrite nth_upto in Hincl by lia.
-    destruct (Znth (Z.of_nat i) lb); inversion Hincl; eauto. }
-  intros (? & ? & b & Hi).
-  eapply derives_trans, bupd_intro.
-  assert (nth i lb None = Some b) as Hi'.
-  { rewrite <- nth_Znth, Nat2Z.id in Hi; auto.
-    rewrite Zlength_correct; lia. }
-  destruct b.
-  erewrite ghost_list_nth with (n := i) by (rewrite nth_map' with (d' := None), Hi'; eauto; lia).
-  rewrite (iter_sepcon_Znth _ _ (Z.of_nat i))
-    by (rewrite Zlength_upto; split; [|apply Nat2Z.inj_lt]; lia).
-  rewrite Znth_upto, Hi by lia.
-  rewrite (sepcon_assoc (agree _ _)), (sepcon_comm (agree _ _)), <- !sepcon_assoc, sepcon_comm, <- !sepcon_assoc, sepcon_assoc.
-  subst; eapply derives_trans; [apply sepcon_derives, agree_join; apply derives_refl|].
-  apply exp_right with l.
-  rewrite !exp_sepcon1; apply exp_right with lg.
-  rewrite !exp_sepcon1; apply exp_right with (replace_nth i lb (Some false)).
-  rewrite prop_true_andp.
-  rewrite (sepcon_comm _ (ghost_master1 _ _)), !sepcon_assoc; apply sepcon_derives.
-  { erewrite map_ext; [apply derives_refl|].
-    intros; simpl.
-    destruct (eq_dec a (Z.of_nat i)); [subst; rewrite Znth_replace_nth | rewrite Znth_replace_nth'];
-      auto; try lia.
-    rewrite Hi; auto. }
-  rewrite sepcon_comm, (sepcon_comm (ghost_list _ _)), !sepcon_assoc; apply sepcon_derives.
-  { rewrite map_replace_nth; auto. }
-  rewrite <- !sepcon_assoc, sepcon_comm, <- !sepcon_assoc.
-  rewrite ghost_set_join, !sepcon_andp_prop1; apply prop_andp_left; intros.
-  rewrite !sepcon_assoc; apply sepcon_derives.
-  { match goal with |- ghost_set _ ?A |-- ghost_set _ ?B =>
-      replace B with A end.
-    apply derives_refl.
-    extensionality; apply prop_ext; split; intro Hin.
-    + inv Hin.
-      * inv H3. rewrite nth_replace_nth; auto; lia.
-      * destruct (eq_dec x i); [subst; rewrite nth_replace_nth | rewrite nth_replace_nth']; auto; lia.
-    +
-      destruct (eq_dec x i); [subst; constructor 1; constructor|].
-      rewrite nth_replace_nth' in Hin; auto; constructor 2; auto. }
-  rewrite <- !sepcon_assoc; apply sepcon_derives, derives_refl.
-  rewrite sepcon_comm, (sepcon_comm _ (iter_sepcon _ _)), <- !sepcon_assoc.
-  rewrite sepcon_assoc; apply sepcon_derives.
-  { rewrite (iter_sepcon_Znth _ (upto _) (Z.of_nat i))
-      by (rewrite Zlength_upto; split; [|apply Nat2Z.inj_lt]; lia).
-    rewrite Znth_upto, Znth_replace_nth by lia.
-    apply sepcon_derives; [apply derives_refl|].
-    erewrite iter_sepcon_func_strong; auto.
-    unfold remove_Znth; intros ? Hin.
-    rewrite Znth_replace_nth'; auto.
-    intro; subst.
-    apply in_app in Hin as [?%In_sublist_upto | ?%In_sublist_upto]; lia.
- }
-  { rewrite sepcon_comm, wand_sepcon_adjoint; apply derives_refl. }
-  { rewrite replace_nth_length; split; auto. }
-  { rewrite !sepcon_assoc, (sepcon_comm (ghost_set _ _)), <- !sepcon_assoc, sepcon_assoc.
-    eapply derives_trans, FF_derives.
-    eapply derives_trans; [apply sepcon_derives; [apply derives_refl|] | rewrite sepcon_comm, FF_sepcon; apply derives_refl].
-    rewrite ghost_set_join; apply prop_andp_left; intros X.
-    inv X. contradiction (H3 i). constructor; auto; constructor. }
-Qed.
-
-(* up *)
-Lemma replace_nth_same' : forall {A} n l (a d : A), nth n l d = a -> replace_nth n l a = l.
-Proof.
-  intros; subst; apply replace_nth_same.
-Qed.
-
-Lemma wsat_close : forall i P,
-  (wsat * invariant i P * |> P * ghost_list g_dis (list_singleton i (Some tt)) |--
-  |==> wsat * ghost_set g_en (Singleton i)).
-Proof.
-  intros; unfold wsat, invariant.
-  rewrite !exp_sepcon1; apply exp_left; intros l.
-  rewrite !exp_sepcon1; apply exp_left; intros lg.
-  rewrite !exp_sepcon1; apply exp_left; intros lb.
-  rewrite !sepcon_andp_prop1; apply prop_andp_left; intros [].
-  rewrite !exp_sepcon2, !exp_sepcon1; apply exp_left; intros g.
-  eapply derives_trans, (prop_andp_left (i < length lg /\ Znth (Z.of_nat i) lg = g /\
-    exists b, Znth (Z.of_nat i) lb = Some b)%nat).
-  { rewrite <- sepcon_assoc, (sepcon_comm _ (ghost_snap _ _)), <- !sepcon_assoc.
-    unfold master_list; rewrite snap_master_join1.
-    rewrite !sepcon_andp_prop1; apply andp_derives, derives_refl.
-    apply prop_derives; intros Hincl.
-    apply list_incl_singleton in Hincl.
-    destruct (lt_dec i (length lg));
-      [|rewrite nth_overflow in Hincl by (rewrite map_length, upto_length; lia); discriminate].
-    rewrite nth_map' with (d' := 0) in Hincl by (rewrite upto_length; lia).
-    rewrite nth_upto in Hincl by lia.
-    destruct (Znth (Z.of_nat i) lb); inversion Hincl; eauto. }
-  intros (? & ? & b & Hi).
-  eapply derives_trans, bupd_intro.
-  assert (nth i lb None = Some b) as Hi'.
-  { rewrite <- nth_Znth, Nat2Z.id in Hi; auto.
-    rewrite Zlength_correct; lia. }
-  destruct b.
-  { rewrite (sepcon_comm (ghost_master1 _ _)), sepcon_comm, <- !sepcon_assoc.
-    rewrite 4sepcon_assoc; eapply derives_trans, FF_derives.
-    eapply derives_trans; [apply sepcon_derives, derives_refl | rewrite FF_sepcon; apply derives_refl].
-    eapply derives_trans; [apply andp_right, derives_refl; apply ghost_valid_2|].
-    apply prop_andp_left; intros (? & J & ?).
-    apply list_join_nth with (n := i) in J.
-    erewrite nth_singleton, nth_map' with (d' := None) in J by lia.
-    rewrite Hi' in J; inv J.
-    inv H7.
-    inv H5. }
-  rewrite ghost_set_remove with (a := i) by auto.
-  apply exp_right with l.
-  rewrite exp_sepcon1; apply exp_right with lg.
-  rewrite exp_sepcon1; apply exp_right with (replace_nth i lb (Some true)).
-  rewrite replace_nth_length, prop_true_andp by auto.
-  rewrite !sepcon_assoc; apply sepcon_derives.
-  { erewrite map_ext; [apply derives_refl|].
-    intros.
-    destruct (eq_dec a (Z.of_nat i)); [subst; rewrite Znth_replace_nth | rewrite Znth_replace_nth'];
-      auto; try lia.
-    rewrite Hi; auto. }
-  rewrite sepcon_comm, sepcon_assoc, sepcon_comm, <- !sepcon_assoc; apply sepcon_derives, derives_refl.
-  rewrite !sepcon_assoc, (sepcon_comm (ghost_list _ _) (_ * _)%pred), <- !sepcon_assoc, sepcon_assoc.
-  apply sepcon_derives.
-  rewrite !sepcon_assoc; apply sepcon_derives.
-  { match goal with |- ghost_set _ ?A |-- ghost_set _ ?B =>
-      replace B with A end; [apply derives_refl|].
-    extensionality; apply prop_ext; split; intro Hin.
-    + inv Hin.
-      destruct (eq_dec x i); [subst; contradiction H4; constructor|].
-      rewrite nth_replace_nth'; auto.
-    +
-      destruct (eq_dec x i); [subst; rewrite nth_replace_nth in Hin by lia; discriminate|].
-      rewrite nth_replace_nth' in Hin by auto; constructor; auto.
-      intros X; inv X; contradiction. }
-  { rewrite (iter_sepcon_Znth _ _ (Z.of_nat i))
-      by (rewrite Zlength_upto; split; [|apply Nat2Z.inj_lt]; lia).
-    rewrite (iter_sepcon_Znth _ (upto _) (Z.of_nat i))
-      by (rewrite Zlength_upto; split; [|apply Nat2Z.inj_lt]; lia).
-    rewrite !Znth_upto, !Znth_replace_nth by lia.
-    rewrite Hi.
-    rewrite (sepcon_comm _ (|> P)%pred), <- !sepcon_assoc, sepcon_comm, <- !sepcon_assoc, sepcon_assoc.
-    subst; eapply derives_trans; [apply sepcon_derives, derives_refl; apply agree_join2|].
-    rewrite (sepcon_comm _ (agree _ _)), !sepcon_assoc; apply sepcon_derives; [apply derives_refl|].
-    rewrite <- sepcon_assoc, sepcon_comm, <- sepcon_assoc; apply sepcon_derives.
-    + rewrite sepcon_comm, wand_sepcon_adjoint; apply derives_refl.
-    + erewrite iter_sepcon_func_strong; eauto.
-      unfold remove_Znth; intros ? Hin.
-      rewrite Znth_replace_nth'; auto.
-      intro; subst.
-      apply in_app in Hin as [?%In_sublist_upto | ?%In_sublist_upto]; lia. }
-  { unfold ghost_list. erewrite <- ghost_op; [apply derives_refl|].
-    rewrite map_replace_nth.
-    apply (list_join_singleton(P := token_PCM)).
-    { rewrite map_length; lia. }
-    rewrite nth_map' with (d' := None) by lia.
-    rewrite Hi'; constructor. }
-Qed.
-
-Lemma invariant_dealloc : forall i P, invariant i P |-- emp.
-Proof.
-  intros; unfold invariant.
-  apply exp_left; intro g.
-  rewrite <- (emp_sepcon emp).
-  apply sepcon_derives; apply ghost_dealloc.
-Qed.
-
-Lemma ghost_is_pred_nonexpansive : forall g H, nonexpansive (fun P => ghost_is (singleton g
-  (existT (fun RA : Ghost => {a : @G RA | valid a}) unit_PCM
-           (exist (fun a : G => valid a) (tt : @G unit_PCM) H),
-        pred_of P))).
-Proof.
-  unfold nonexpansive.
-  intros ??????; split; intros ?????; simpl in *;
-    match goal with H : join_sub ?a ?b |- join_sub ?c ?b =>
-      assert (a = c) as <-; auto end; simpl;
-    rewrite !ghost_fmap_singleton; do 2 f_equal; simpl; f_equal;
-    extensionality; apply pred_ext; intros ? []; split; auto;
-    eapply H0; try apply necR_refl; auto; apply necR_level in H2; apply ext_level in H3; lia.
-Qed.
-
-Lemma agree_nonexpansive : forall g, nonexpansive (agree g).
-Proof.
-  intros; unfold agree, own.
-  apply exists_nonexpansive; intros.
-  unfold Own.
-  apply conj_nonexpansive; [apply const_nonexpansive|].
-  apply ghost_is_pred_nonexpansive.
-Qed.
-
-Lemma invariant_nonexpansive : forall N, nonexpansive (invariant N).
-Proof.
-  intros; unfold invariant.
-  apply exists_nonexpansive; intros.
-  apply sepcon_nonexpansive.
-  - apply const_nonexpansive.
-  - apply agree_nonexpansive.
-Qed.
-
-Lemma ghost_is_pred_nonexpansive2 : forall g H f,
-    nonexpansive f ->
-    nonexpansive (fun P => ghost_is (singleton g
-  (existT (fun RA : Ghost => {a : @G RA | valid a}) unit_PCM
-           (exist (fun a : G => valid a) (tt : @G unit_PCM) H),
-        pred_of (f P)))).
-Proof.
-  unfold nonexpansive.
-  intros ??????; split; intros ?????; specialize (H0 _ _ _ H1);
-  simpl in *; match goal with H : join_sub ?a ?b |- join_sub ?c ?b =>
-      assert (a = c) as <-; auto end; simpl;
-    rewrite !ghost_fmap_singleton; do 2 f_equal; simpl; f_equal;
-    extensionality; apply pred_ext; intros ? []; split; auto;
-    eapply H0; try apply necR_refl; auto; apply necR_level in H3; apply ext_level in H4; lia.
-Qed.
-
-Lemma agree_nonexpansive2 : forall g f,
-    nonexpansive f -> nonexpansive (fun a => agree g (f a)).
-Proof.
-  intros; unfold agree, own.
-  apply exists_nonexpansive; intros.
-  unfold Own.
-  apply conj_nonexpansive; [apply const_nonexpansive|].
-  now apply ghost_is_pred_nonexpansive2.
-Qed.
-
-Lemma invariant_nonexpansive2 : forall N f,
-    nonexpansive f -> nonexpansive (fun a => invariant N (f a)).
-Proof.
-  intros; unfold invariant.
-  apply exists_nonexpansive; intros.
-  apply sepcon_nonexpansive.
-  - apply const_nonexpansive.
-  - now apply agree_nonexpansive2.
-Qed.
-
-(* Consider putting rules for invariants and fancy updates in msl (a la ghost_seplog), and proofs
-   in veric (a la own). *)
-
-Lemma ghost_set_empty : forall g s,
-  (ghost_set g s = ghost_set g s * ghost_set g (Empty_set))%pred.
-Proof.
-  intros.
-  apply ghost_op.
-  hnf; split.
-  - constructor.
-    intros ? X; inv X.
-    inv H0.
-  - extensionality; apply prop_ext; split; intro X; [left | inv X]; auto.
-    inv H.
-Qed.
-
-Lemma wsat_empty_eq : (wsat = wsat * ghost_set g_en (Empty_set))%pred.
-Proof.
-  unfold wsat.
-  repeat (rewrite exp_sepcon1; f_equal; extensionality).
-  rewrite !sepcon_andp_prop1; f_equal.
-  rewrite !sepcon_assoc; f_equal; f_equal.
-  rewrite !(sepcon_comm (ghost_set _ _)), sepcon_assoc; f_equal.
-  rewrite sepcon_comm; apply ghost_set_empty.
-Qed.
-
-End Invariants.
-
-Lemma make_wsat : emp |-- |==> EX inv_names : invG, wsat.
-Proof.
-  unfold wsat.
-  eapply derives_trans with (Q := (_ * emp)%pred); [rewrite sepcon_emp; apply (ghost_alloc(RA := snap_PCM(ORD := list_order gname)) (Tsh, nil) NoneP); simpl; auto|].
-  eapply derives_trans; [apply bupd_frame_r | eapply derives_trans, bupd_trans; apply bupd_mono].
-  rewrite exp_sepcon1; apply exp_left; intro g_inv.
-  eapply derives_trans; [eapply sepcon_derives with (q' := (|==> _ * emp)%pred); [apply derives_refl |
-    rewrite sepcon_emp; apply (ghost_alloc(RA := list_PCM (exclusive_PCM unit)) nil NoneP); simpl; auto]|].
-  eapply derives_trans; [apply bupd_frame_l | eapply derives_trans, bupd_trans; apply bupd_mono].
-  rewrite exp_sepcon1, exp_sepcon2; apply exp_left; intro g_dis.
-  rewrite <- sepcon_assoc.
-  eapply derives_trans; [eapply sepcon_derives with (q' := (|==> _ * emp)%pred); [apply derives_refl |
-    rewrite sepcon_emp; apply (ghost_alloc(RA := set_PCM) Ensembles.Empty_set NoneP); simpl; auto]|].
-  eapply derives_trans; [apply bupd_frame_l | eapply derives_trans, bupd_trans; apply bupd_mono].
-  rewrite exp_sepcon1, !exp_sepcon2; apply exp_left; intro g_en.
-  rewrite <- sepcon_assoc.
-  eapply derives_trans, bupd_intro.
-  apply exp_right with {| g_inv := g_inv; g_dis := g_dis; g_en := g_en |}, exp_right with nil, exp_right with nil, exp_right with nil; simpl.
-  rewrite !sepcon_andp_prop1; apply andp_right.
-  - hnf; intros; simpl; auto.
-  - repeat apply sepcon_derives; auto.
-    replace (fun i : iname => match i with
-                                     | 0%nat | _ => None
-                                     end = Some false) with (@Ensembles.Empty_set nat); auto.
-    extensionality; apply prop_ext; split; intro H.
-    + inv H.
-    + hnf in H.
-      destruct x; inv H.
-Qed.
